```litex
"""
prove:
    fn_template f(x, y R):
        dom:
            x > 1
        fn (a, b R) R:
            dom:
                a = x
            =>:
                f(a, b) = y

    fn_template g(x, y R):
        fn (a, b R) R:
            dom:
                a = x
            =>:
                g(a, b) = y

    let f2 g(1,2)

    f2 $in g(1,2)

    forall a,b R:
        a = 1
        =>:
            f2(a, b) = 2

prove:
    fn_template seq3(s set):
        fn (n N) s

    fn g(x N) R

    let t seq3(R)

    t $in seq3(R)

    g $in fn(N)R

    g $in seq3(R)

    fn_template seq2(s set):
        fn (n N) s:
            dom:
                n > 3

    fn g2(n N) R:
        dom:
            n > 1

    know forall n N: n > 3 => n > 1

    g2 $in seq2(R)

prove:
    fn_template dom_R_R_ret_R():
        fn (x, y R) R

    $in(+, dom_R_R_ret_R())
    $in(-, dom_R_R_ret_R())

    fn_template dom_R_ret_R():
        fn (x R) R:
            dom_R_ret_R(x) = -1 * x

    fn reverse(x R) R:
        reverse(x) = - x

    forall x R:
        reverse(x) = - x
        reverse(x) = -1 * x

    $in(reverse, dom_R_ret_R())

prove:
    fn_template f_template():
        fn (x Z) Z:
            dom:
                x >= -1
            =>:
                f_template(x) = x + 1  

    let m f_template()
    m(0) = 0 + 1

    # prove xxx $in fn_template
    fn f2(x Z) Z:
        dom:
            x >= -1
        =>:
            f2(x) = x + 1

    f2 $in f_template()

    # fn name as fn name
    fn f3(x Z) f_template:
        dom:
            x > 0 
    know f3(1) $in f_template() # true, because return value of f3 is $in f_template。这是要写的，否则找不到f3(1) 的性质
    f3(1)(2) = 2 + 1

prove:
    fn fn_add(f fn(R)R, g fn(R)R) fn(R,R)R => forall x R, y R => fn_add(f, g)(x, y) = f(x) + g(y)

    fn f(x R) R => f(x) = x
    fn_add(f, f) $in fn(R,R)R

    fn_add(f, f)(1, 2) = f(1) + f(2)

    """
```
