```litex
claim:
    forall a, b, x R:
        x^2 + 2 * a * x + b = 0
        a^2 - b >= 0
        =>:
            x = -a + sqrt(a^2 - b) or x = -a - sqrt(a^2 - b)
    prove:
        sqrt(a^2 - b) * sqrt(a^2 - b) = sqrt(a^2 - b) ^ 2 = a^2 - b
        (x + a - sqrt(a^2 - b)) * (x + a + sqrt(a^2 - b)) = x ^ 2 + 2 * a * x + a^2 - sqrt(a^2 - b) ^ 2 = x ^ 2 + 2 * a * x + a^2 - (a^2 - b) = x ^ 2 + 2 * a * x + b = 0
        $product_is_0_then_at_least_one_factor_is_0(x + a - sqrt(a^2 - b), x + a + sqrt(a^2 - b))
        
        prove_case_by_case:
            =>:
                x = -a + sqrt(a^2 - b) or x = -a - sqrt(a^2 - b)
            case x + a + sqrt(a^2 - b) = 0:
                x + a + sqrt(a^2 - b) + (-a - sqrt(a^2 - b)) = 0 + (-a - sqrt(a^2 - b))
                x = 0 + (-a - sqrt(a^2 - b))
                x = -a - sqrt(a^2 - b) 
            case x + a - sqrt(a^2 - b) = 0:
                x + a - sqrt(a^2 - b) + (-a + sqrt(a^2 - b)) = 0 + (-a + sqrt(a^2 - b))
                x = 0 + (-a + sqrt(a^2 - b))
                x = -a + sqrt(a^2 - b)
```
