```litex
claim:
    forall x, y R:
        abs(x + y) <= abs(x) + abs(y)
    prove:
        prove_in_each_case:
            or:
                x >= 0
                x < 0
            =>:
                abs(x + y) <= abs(x) + abs(y)
            prove:
                x >= 0
                prove_in_each_case:
                    or:
                        y >= 0
                        y < 0
                    =>:
                        abs(x + y) <= abs(x) + abs(y)
                    prove:
                        y >= 0
                        abs(x) = x
                        abs(y) = y
                        x + y >= 0
                        abs(x + y) = x + y
                        abs(x + y) = abs(x) + abs(y)
                        abs(x + y) <= abs(x) + abs(y)
                    prove:
                        y < 0
                        abs(x) = x
                        abs(y) = -y
                        prove_in_each_case:
                            or:
                                x + y >= 0
                                x + y < 0
                            =>:
                                abs(x + y) <= abs(x) + abs(y)
                            prove:
                                x + y >= 0
                                abs(x + y) = x + y
                                y < 0
                                x + y < x
                                x + y <= x
                                -y > 0
                                y < 0
                                x + (-y) > x
                                x < x + (-y)
                                x + y < x
                                x + y <= x + (-y)
                                abs(x + y) <= abs(x) + abs(y)
                            prove:
                                x + y < 0
                                abs(x + y) = -(x + y) = -x - y
                                x >= 0
                                -x <= 0
                                -x - y <= 0 -y
                                -x - y <= -y
                                -y <= x + (-y)
                                -x - y <= x + (-y)
                                abs(x + y) <= abs(x) + abs(y)
            prove:
                x < 0
                prove_in_each_case:
                    or:
                        y >= 0
                        y < 0
                    =>:
                        abs(x + y) <= abs(x) + abs(y)
                    prove:
                        y >= 0
                        abs(x) = -x
                        abs(y) = y
                        prove_in_each_case:
                            or:
                                x + y >= 0
                                x + y < 0
                            =>:
                                abs(x + y) <= abs(x) + abs(y)
                            prove:
                                x + y >= 0
                                abs(x + y) = x + y
                                x < 0
                                x + y < y
                                x + y <= y
                                -x > 0
                                -x >= 0
                                (-x) + y > y
                                x + y < y
                                x + y <= y
                                x + y <= (-x) + y
                                abs(x + y) <= abs(x) + abs(y)
                            prove:
                                x + y < 0
                                abs(x + y) = -(x + y) = -x - y
                                y >= 0
                                -y <= 0
                                -x - y <= -x
                                -x - y <= (-x) + y
                                abs(x + y) <= abs(x) + abs(y)
                    prove:
                        y < 0
                        abs(x) = -x
                        abs(y) = -y
                        x + y < y
                        y < 0
                        x + y < 0
                        abs(x + y) = -(x + y) = -x - y
                        abs(x + y) = -x + (-y) = abs(x) + abs(y)
                        abs(x + y) <= abs(x) + abs(y)


```
